Add cx

src/statics.lean
@@ -1,12 +1,24 @@
 import syntax
 
-inductive has_typ: exp -> typ -> Prop
-| int (n: ℤ): has_typ (exp.int n) typ.int
-| true: has_typ exp.true typ.bool
-| false: has_typ exp.false typ.bool
+inductive cx: Type
+| nil: cx
+| cons: cx -> var -> typ -> cx
+
+inductive lookup: cx -> var -> typ -> Prop
+| hd (Γ: cx) (x: var) (τ: typ): lookup (cx.cons Γ x τ) x τ
+| tl (Γ: cx) (x: var) (y: var) (τ: typ) (τ': typ):
+    x ≠ y ->
+    lookup Γ x τ ->
+    lookup (cx.cons Γ y τ') x τ
+
+inductive has_typ: cx -> exp -> typ -> Prop
+| int (Γ: cx) (n: ℤ): has_typ Γ (exp.int n) typ.int
+| true (Γ: cx): has_typ Γ exp.true typ.bool
+| false (Γ: cx): has_typ Γ exp.false typ.bool
 | if_
+    (Γ: cx)
     (e1: exp) (e2: exp) (e3: exp) (τ: typ):
-    has_typ e1 typ.bool ->
-    has_typ e2 τ ->
-    has_typ e3 τ ->
-    has_typ (exp.if_ e1 e2 e3) τ
+    has_typ Γ e1 typ.bool ->
+    has_typ Γ e2 τ ->
+    has_typ Γ e3 τ ->
+    has_typ Γ (exp.if_ e1 e2 e3) τ
