src/safety.lean
@@ -1,45 +1,50 @@
 import helpers
 
+-- seems like we have to write this as taking in a general context and also a
+-- proof that it is nil, rather than just having `typing: has_typ cx.nil e tau`.
 theorem progress
+  (Γ: cx)
   (e: exp) (τ: typ)
-  (typing: has_typ e τ)
+  (is_nil: Γ = cx.nil)
+  (typing: has_typ Γ e τ)
   : val e ∨ (∃ (e': exp), steps e e') :=
 begin
   induction typing,
   left,
-  exact val.int typing,
+  exact val.int typing_n,
   left,
   exact val.true,
   left,
   exact val.false,
   right,
-  cases typing_ih_a,
-  cases bool_canonical_forms typing_e1 typing_a typing_ih_a,
+  cases typing_ih_a is_nil,
+  cases bool_canonical_forms typing_Γ typing_e1 typing_a h,
   existsi typing_e2,
-  rewrite h,
+  rewrite h_1,
   exact steps.if_e2 typing_e2 typing_e3,
   existsi typing_e3,
-  rewrite h,
+  rewrite h_1,
   exact steps.if_e3 typing_e2 typing_e3,
-  cases typing_ih_a,
-  existsi (exp.if_ typing_ih_a_w typing_e2 typing_e3),
-  exact steps.if_e1 typing_e1 typing_ih_a_w typing_e2 typing_e3 typing_ih_a_h,
+  cases h,
+  existsi exp.if_ h_w typing_e2 typing_e3,
+  exact steps.if_e1 typing_e1 h_w typing_e2 typing_e3 h_h,
 end
 
 theorem preservation
-  (e: exp) (e': exp) (τ: typ)
-  (typing: has_typ e τ)
+  (Γ: cx) (e: exp) (e': exp) (τ: typ)
+  (typing: has_typ Γ e τ)
+  (is_nil: Γ = cx.nil)
   (stepping: steps e e')
-  : has_typ e' τ :=
+  : has_typ Γ e' τ :=
 begin
-  induction stepping generalizing τ,
-  let inv := inversion_if stepping_e1 stepping_e2 stepping_e3 τ typing,
-  apply has_typ.if_ stepping_e1' stepping_e2 stepping_e3 τ,
-  exact stepping_ih typ.bool inv.left,
+  induction stepping generalizing Γ τ,
+  let inv := inversion_if Γ stepping_e1 stepping_e2 stepping_e3 τ typing,
+  apply has_typ.if_ Γ stepping_e1' stepping_e2 stepping_e3 τ,
+  exact stepping_ih Γ typ.bool inv.left is_nil,
   exact inv.right.left,
   exact inv.right.right,
-  let inv := inversion_if exp.true stepping_e2 stepping_e3 τ typing,
+  let inv := inversion_if Γ exp.true stepping_e2 stepping_e3 τ typing,
   exact inv.right.left,
-  let inv := inversion_if exp.false stepping_e2 stepping_e3 τ typing,
+  let inv := inversion_if Γ exp.false stepping_e2 stepping_e3 τ typing,
   exact inv.right.right,
 end
