src/syntax.lean
@@ -1,9 +1,11 @@
+def var: Type := string
+
+inductive typ: Type
+| int: typ
+| bool: typ
+
 inductive exp: Type
 | int: ℤ -> exp
 | true: exp
 | false: exp
 | if_: exp -> exp -> exp -> exp
-
-inductive typ: Type
-| int: typ
-| bool: typ
